\section{Product Rule}
\subsection{Product Rule}
	If $f$ and $g$ are differentiable at $x$ then so is $fg$ and:
	\[\left( f(x)g(x) \right)' = f'(x)g(x) + f(x)g'(x)\]
	\[(fg)' = f'g + fg'\]
\subsection{Product of Three Functions}
	If $f$, $g$, and $h$ are differentiable at $x$ then so is $fgh$ and:
	\[(fgh)' = f'gh + fg'h + fgh'\]
\subsection{Generalized Power Rule} 
	If $f$ is differentiable at $x$, then so is $f^n$ and:
	\[\left( \left( f(x) \right)^n \right) = n \left( f(x) \right)^{n-1} f'(x)\]
	\[\left( f^n \right)' = nf^{n-1}f'\]
