\section{Derivative of Trigonometric Functions}
\subsection{Review of Trigonometric Functions}\label{subsec:5.4:trig}
	\[\sin(x) \from \real \to [-1,1]\]
	\[\cos(x) \from \real \to [-1,1]\]
	\[\tan(x) \from \left\{\real \setminus \left\{\frac{\pi}{2} + n\pi \such n \in \integer\right\}\right\} \to \real\]

	\[\sin(x + 2\pi) = \sin(x)\]
	\[\cos(x + 2\pi) = \cos(x)\]

	\[\sin^2(x) + \cos^2(x) = 1\]

	\[\sin(a + b) = \sin(a)\cos(b) + \cos(a)\sin(b)\]
	\[\cos(a + b) = \cos(a)\cos(b) - \sin(a)\sin(b)\]

	\[\sin\left(x + \frac{\pi}{2}\right) = \cos(x)\]
	\[\sin(2x) = 2\sin(x)\cos(x)\]
	\[\cos(2x) = \cos^2(x) - \sin^2(x)\]
	\[\tan(x) = \frac{\sin(x)}{\cos(x)}\]

	\begin{equation}\label{eq:5.4:sinLim}
		\lim_{x \to 0} \frac{\sin x}{x} = 1
	\end{equation}
	\begin{equation}\label{eq:5.4:cosLim}
		\lim_{x \to 0} \frac{\cos x - 1}{x} = 0
	\end{equation}
\subsection{Derivative of $\sin(x)$}
	\[(\sin x)' = \cos x\]
	\[\od{}{x}\sin x = \cos x\]
	\begin{proof}
		\begin{align*}
			(\sin x)' &= \lim_{h \to 0} \frac{\sin(x+h) - \sin(x)}{h}\\
			(\sin x)' &= \lim_{h \to 0} \frac{\sin(x)\cos(h) + \cos(x)\sin(h) - \sin(x)}{h}\\
			(\sin x)' &= \lim_{h \to 0} \frac{\sin(x)\cos(h) - \sin(x)}{h} + \lim_{h \to 0} \frac{\cos(x)\sin(h)}{h}\\
			(\sin x)' &= \sin(x) \lim_{h \to 0}\frac{\cos(h) - 1}{h} + \cos(x)\lim_{h \to 0}\frac{\sin(h)}{h}
		\end{align*}
		Now, using the limits \eqref{eq:5.4:sinLim} and \eqref{eq:5.4:cosLim}:
		\begin{align*}
			(\sin x)' &= sin(x) \times 0 + \cos(x) \times 1\\
			(\sin x)' &= \cos(x)
		\end{align*}
	\end{proof}
\subsection{Derivative of $\sin\left(f(x)\right)$}
	By using the chain rule:
	\[\left( \sin\left( f(x) \right)\right)' = \left(\cos\left( f(x) \right)\right)f'(x)\]
\subsection{Derivative of $\cos x$}
	\[(\cos x)' = -\sin x\]
\subsection{Derivative of $\cos \left( f(x) \right)$}
	By using the chain rule:
	\[\left( \cos \left( f(x) \right) \right)' = -\left(\sin \left( f(x) \right) \right) f'(x)\]
\subsection{Derivative of $\tan x$}
	\[(\tan x)' = \frac{1}{\cos^2 x} = \sec^2 x\]
