\chapter{Equations}
	\paragraph{Fundamental Limits}
		\[\lim_{h \to 0} \frac{\sin h}{h} = 1\]
		\[\lim_{h \to 0} \frac{\cos h - 1}{h} = 0\]
		\[\lim_{h \to 0} \frac{\e^h - 1}{h} = 1\]
	\paragraph{Deriving Rules}
		\[(x^n)' = nx^{n-1}\]
		\[\left(\frac{a}{x^n}\right)' = -\frac{na}{x^{n+1}}\]
		\[(\sqrt{x})' = \frac{1}{2\sqrt{x}}\]
		\[[f(x) \pm g(x)]' = f'(x) \pm g'(x)\]

		\[(fg)' = f'g + fg'\]
		\[(f^n)' = nf^{n-1}f'\]

		\[\left(\frac{f}{g}\right)' = \frac{f'g - fg'}{g^2}\]

		\[(f \circ g)'(x) = f'(g(x))g'(x)\]
	\paragraph{Tangent Line}
		\[m = f'(a)\]
		\[y - f(a) = m(x-a) \quad \equiv \quad y = m(x-a) + f(a)\]
	\paragraph{Logarithms}
		\[b^x = y \quad \equiv \quad x = \log_b y\]
		\[\log_b x^n = n\log_b x\]
		\[\log_b(xy) = \log_b x + \log_b y\]
		\[\log_b\left(\frac{x}{y}\right) = \log_b x - \log_b y\]
		\[\log_a(x) = \frac{\log_b x}{\log_b a}\]
		\[a^x = b^{x\log_b a}\]
	\paragraph{Vectors}
		\[\vv{a} \cdot \vv{b} = \|\vv{a}\|\|\vv{b}\|\cos\theta\]
		\[\vv{a} \times \vv{b} = \|\vv{a}\|\|\vv{b}\|\sin\theta\]
		\[SProj_{\vv{b}}\vv{a} = \|\vv{a}\|\cos\theta = \frac{\vv{a} \cdot \vv{b}}{\|\vv{b}\|}\]
		\[VProj_{\vv{b}}\vv{a} = SProj_{\vv{b}}\vv{a}\hat{b} = \frac{(\vv{a} \cdot \vv{b})\vv{b}}{\|\vv{b}\|^2}\]
		\[\cos\theta = \frac{\vv{a}\cdot\vv{b}}{\|\vv{a}\|\|\vv{b}\|}\]
	\vspace{2cm}
	\begin{center}
		\Huge
		Pray to Gugoiu and it will be okay!
	\end{center}
