\section{Basics}
\paragraph{Dot product}
	\begin{equation}
		\vv{a} \cdot \vv{b} = \norm{a} \norm{b} \cos \theta
	\end{equation}
	\begin{equation}
		\vv{a} \cdot \vv{b} = a_xb_x + a_yb_y + a_zb_z
	\end{equation}
\paragraph{Cross product}
	\begin{equation}
		\norm{\vv{a} \times \vv{b}} = \norm{a} \norm{b} \sin \theta
	\end{equation}
	\begin{equation}
		\vv{a} \times \vv{b} = \vv{i}(a_yb_z - a_zb_y) - \vv{j}(a_xb_z - a_zb_x) + \vv{k}(a_xb_y - a_yb_x)
	\end{equation}
	\begin{equation}
		\vv{a} \times \vv{b} = (a_yb_z - a_zb_y, -a_xb_z + a_zb_x, a_xb_y - a_yb_x)
	\end{equation}
\paragraph{Limit}
	\begin{equation}
		f'(x) = \lim_{h \to 0}\frac{f(x+h) - f(x)}{h}
	\end{equation}
	\begin{equation}
		f'(x) = \lim_{h \to 0}\frac{f(x+h) - f(x - h)}{2h}
	\end{equation}
	\begin{equation}
		f'(x) = \lim_{u \to x}\frac{f(u) - f(x)}{u-x}
	\end{equation}
\paragraph{Tangent line}
	\begin{equation}
		y = f'(a)(x-a) + f(a)
	\end{equation}
